Work on the template adequacy theorem(s)

theories/examples/template_adequacy.v
@@ -7,34 +7,26 @@ From cap_machine Require Import
      rules logrel fundamental.
 From cap_machine.examples Require Import addr_reg_sample mkregion_helpers.
 
-Record initial_prog := MkInitialProg {
+Record prog := MkProg {
   prog_start: Addr;
   prog_end: Addr;
-  prog: list Word;
+  prog_instrs: list Word;
 
   prog_size:
-    (prog_start + length prog)%a = Some prog_end;
+    (prog_start + length prog_instrs)%a = Some prog_end;
 }.
 
-Definition prog_region (P: initial_prog): gmap Addr Word :=
-  mkregion (prog_start P) (prog_end P) (prog P).
+Definition prog_region (P: prog): gmap Addr Word :=
+  mkregion (prog_start P) (prog_end P) (prog_instrs P).
 
-Definition is_initial_registers (P: initial_prog) (reg: gmap RegName Word) :=
-  reg !! PC = Some (WCap RWX (prog_start P) (prog_end P) (prog_start P)) ∧
-  (∀ (r: RegName), r ∉ ({[ PC ]} : gset RegName) →
-     ∃ (w:Word), reg !! r = Some w ∧ is_cap w = false).
-
-Lemma initial_registers_full_map (P: initial_prog) reg :
-  is_initial_registers P reg →
-  (∀ r, is_Some (reg !! r)).
+Lemma prog_region_dom (P: prog):
+  dom (gset Addr) (prog_region P) =
+  list_to_set (region_addrs (prog_start P) (prog_end P)).
 Proof.
-  intros (HPC & Hothers) r.
-  destruct (decide (r = PC)) as [->|]. by eauto.
-  destruct (Hothers r) as (w & ? & ?); [| eauto]. set_solver.
+  rewrite /prog_region /mkregion dom_list_to_map_L fst_zip //.
+  rewrite region_addrs_length /region_size.
+  pose proof (prog_size P). solve_addr.
 Qed.
-
-Definition is_initial_memory (P: initial_prog) (m: gmap Addr Word) :=
-  prog_region P ⊆ m.
 
 Record memory_inv := MkMemoryInv {
   minv : gmap Addr Word → Prop;
@@ -82,10 +74,42 @@ Proof.
   eapply Hsub; eauto.
 Qed.
 
+Lemma filter_dom_is_dom (m: gmap Addr Word) (d: gset Addr):
+  d ⊆ dom (gset Addr) m →
+  dom (gset Addr) (filter (λ '(a, _), a ∈ d) m) = d.
+Proof.
+  intros Hd. eapply set_eq. intros a.
+  rewrite (dom_filter_L _ _ d); auto.
+  intros. split; intros H.
+  { rewrite elem_of_subseteq in Hd |- * => Hd. specialize (Hd _ H).
+    eapply elem_of_gmap_dom in Hd as [? ?]. eexists. split; eauto. }
+  { destruct H as [? [? ?] ]; auto. }
+Qed.
+
 Definition minv_sep `{memG Σ} (I: memory_inv): iProp Σ :=
   ∃ (m: gmap Addr Word),
     ([∗ map] a↦w ∈ m, a ↦ₐ w) ∗ ⌜dom (gset Addr) m = minv_dom I⌝ ∗
     ⌜minv I m⌝.
+
+
+Module basic.
+
+Definition is_initial_registers (P: prog) (reg: gmap RegName Word) :=
+  reg !! PC = Some (WCap RWX (prog_start P) (prog_end P) (prog_start P)) ∧
+  (∀ (r: RegName), r ∉ ({[ PC ]} : gset RegName) →
+     ∃ (w:Word), reg !! r = Some w ∧ is_cap w = false).
+
+Lemma initial_registers_full_map (P: prog) reg :
+  is_initial_registers P reg →
+  (∀ r, is_Some (reg !! r)).
+Proof.
+  intros (HPC & Hothers) r.
+  destruct (decide (r = PC)) as [->|]. by eauto.
+  destruct (Hothers r) as (w & ? & ?); [| eauto]. set_solver.
+Qed.
+
+Definition is_initial_memory (P: prog) (m: gmap Addr Word) :=
+  prog_region P ⊆ m.
 
 Section Adequacy.
   Context (Σ: gFunctors).
@@ -95,7 +119,7 @@ Section Adequacy.
   Context {na_invg: na_invG Σ}.
   Context `{MP: MachineParameters}.
 
-  Context (P: initial_prog).
+  Context (P: prog).
   Context (I : memory_inv).
 
   Definition invN : namespace := nroot .@ "templateadequacy" .@ "inv".
@@ -146,27 +170,11 @@ Section Adequacy.
 
     iMod (inv_alloc invN ⊤ (minv_sep I) with "[Hprog_inv]") as "#Hinv".
     { iNext. unfold minv_sep. iExists prog_in_inv. iFrame. iPureIntro.
-      assert (dom (gset Addr) prog_in_inv = minv_dom I) as Hi_dom.
-      { eapply set_eq. intros a. rewrite /prog_in_inv.
-        set prog_addrs := region_addrs (prog_start P) (prog_end P).
-        set inv_addrs := filter (λ a, a ∈ minv_dom I) prog_addrs.
-        set inv_addrs_s := (list_to_set inv_addrs : gset Addr).
-        rewrite (dom_filter_L _ _ inv_addrs_s).
-        2: { intros a'. rewrite /inv_addrs_s /inv_addrs /prog_addrs.
-             rewrite elem_of_list_to_set elem_of_list_filter. split.
-             { intros [? ?].
-               assert (is_Some (prog_region P !! a')) as [? ?].
-               { apply elem_of_gmap_dom. rewrite dom_mkregion_eq. 2: by apply prog_size.
-                 rewrite elem_of_list_to_set //. }
-               eexists. split; eauto. }
-             { intros [? (? & ?)]. split; auto.
-               eapply in_dom_mkregion, elem_of_gmap_dom. eauto. } }
-        rewrite /inv_addrs_s /inv_addrs elem_of_list_to_set elem_of_list_filter.
-        split; intros; destruct_and?; split_and?; eauto.
-        pose proof (proj1 (elem_of_subseteq _ _) HIdom a) as HH.
-        rewrite elem_of_list_to_set in HH |- * => HH. eauto. }
-      split; auto; []. eapply minv_sub_restrict; [ | | eapply HI].
-      by rewrite Hi_dom //. transitivity (prog_region P); auto. rewrite /prog_in_inv.
+      assert (minv_dom I ⊆ dom (gset Addr) (prog_region P)).
+      { etransitivity. eapply HIdom. rewrite prog_region_dom//. }
+      rewrite filter_dom_is_dom; auto. split; auto.
+      eapply minv_sub_restrict; [ | | eapply HI]. rewrite filter_dom_is_dom//.
+      transitivity (prog_region P); auto. rewrite /prog_in_inv.
       eapply map_filter_sub; typeclasses eauto. }
 
     unfold is_initial_registers in Hreg.
@@ -205,7 +213,7 @@ Section Adequacy.
 End Adequacy.
 
 Theorem template_adequacy `{MachineParameters}
-    (P: initial_prog) (I: memory_inv)
+    (P: prog) (I: memory_inv)
     (m m': Mem) (reg reg': Reg) (es: list cap_lang.expr):
   is_initial_memory P m →
   is_initial_registers P reg →
@@ -228,3 +236,179 @@ Proof.
               na_invΣ]).
   intros. eapply (@template_adequacy' Σ); eauto; typeclasses eauto.
 Qed.
+
+End basic.
+
+Module with_adv.
+
+Definition is_initial_registers (P Adv: prog) (reg: gmap RegName Word) :=
+  reg !! PC = Some (WCap RWX (prog_start P) (prog_end P) (prog_start P)) ∧
+  reg !! r_t0 = Some (WCap RWX (prog_start Adv) (prog_end Adv) (prog_start Adv)) ∧
+  (∀ (r: RegName), r ∉ ({[ PC ]} : gset RegName) →
+     ∃ (w:Word), reg !! r = Some w ∧ is_cap w = false).
+
+Lemma initial_registers_full_map (P Adv: prog) reg :
+  is_initial_registers P Adv reg →
+  (∀ r, is_Some (reg !! r)).
+Proof.
+  intros (HPC & Hr0 & Hothers) r.
+  destruct (decide (r = PC)) as [->|]. by eauto.
+  destruct (decide (r = r_t0)) as [->|]. by eauto.
+  destruct (Hothers r) as (w & ? & ?); [| eauto]. set_solver.
+Qed.
+
+Definition is_initial_memory (P Adv: prog) (m: gmap Addr Word) :=
+  prog_region P ⊆ m
+  ∧ prog_region Adv ⊆ m
+  ∧ prog_region P ##ₘ prog_region Adv.
+
+Section Adequacy.
+  Context (Σ: gFunctors).
+  Context {inv_preg: invPreG Σ}.
+  Context {mem_preg: gen_heapPreG Addr Word Σ}.
+  Context {reg_preg: gen_heapPreG RegName Word Σ}.
+  Context {na_invg: na_invG Σ}.
+  Context `{MP: MachineParameters}.
+
+  Context (P Adv: prog).
+  Context (I : memory_inv).
+
+  Definition invN : namespace := nroot .@ "templateadequacy" .@ "inv".
+
+  Lemma template_adequacy' (m m': Mem) (reg reg': Reg) (es: list cap_lang.expr):
+    is_initial_memory P Adv m →
+    is_initial_registers P Adv reg →
+    Forall (λ w, is_cap w = false) (prog_instrs Adv) →
+    minv I m →
+    minv_dom I ⊆ list_to_set (region_addrs (prog_start P) (prog_end P)) →
+
+    let prog_map := filter (fun '(a, _) => a ∉ minv_dom I) (prog_region P) in
+    (∀ `{memG Σ, regG Σ, logrel_na_invs Σ} rmap,
+     dom (gset RegName) rmap = all_registers_s ∖ {[ PC; r_t0 ]} →
+     ⊢ inv invN (minv_sep I)
+       ∗ PC ↦ᵣ WCap RWX (prog_start P) (prog_end P) (prog_start P)
+       ∗ r_t0 ↦ᵣ WCap RWX (prog_start Adv) (prog_end Adv) (prog_start Adv)
+       ∗ interp (WCap RWX (prog_start Adv) (prog_end Adv) (prog_start Adv))
+       ∗ ([∗ map] r↦w ∈ rmap, r ↦ᵣ w ∗ ⌜is_cap w = false⌝)
+       ∗ ([∗ map] a↦w ∈ prog_map, a ↦ₐ w)
+       -∗ WP Seq (Instr Executable) {{ λ _, True }}) →
+
+    rtc erased_step ([Seq (Instr Executable)], (reg, m)) (es, (reg', m')) →
+    minv I m'.
+  Proof.
+    intros Hm Hreg Hadv HI HIdom prog_map Hspec Hstep.
+    pose proof (@wp_invariance Σ cap_lang _ NotStuck) as WPI. cbn in WPI.
+    pose (fun (c:ExecConf) => minv I c.2) as state_is_good.
+    specialize (WPI (Seq (Instr Executable)) (reg, m) es (reg', m') (state_is_good (reg', m'))).
+    eapply WPI. intros Hinv κs. clear WPI.
+
+    unfold is_initial_memory in Hm.
+
+    iMod (gen_heap_init (m:Mem)) as (mem_heapg) "(Hmem_ctx & Hmem & _)".
+    iMod (gen_heap_init (reg:Reg)) as (reg_heapg) "(Hreg_ctx & Hreg & _)" .
+    iMod (@na_alloc Σ na_invg) as (logrel_nais) "Hna".
+
+    pose memg := MemG Σ Hinv mem_heapg.
+    pose regg := RegG Σ Hinv reg_heapg.
+    pose logrel_na_invs := Build_logrel_na_invs _ na_invg logrel_nais.
+
+    specialize (Hspec memg regg logrel_na_invs).
+    destruct Hm as (HM & HA & Hdisj).
+
+    iDestruct (big_sepM_subseteq with "Hmem") as "Hprogadv".
+    { transitivity (prog_region P ∪ prog_region Adv); eauto.
+      rewrite map_subseteq_spec. intros * HH.
+      apply lookup_union_Some in HH; auto. destruct HH as [HH|HH].
+      eapply map_subseteq_spec in HM; eauto.
+      eapply map_subseteq_spec in HA; eauto. }
+    iDestruct (big_sepM_union with "Hprogadv") as "[Hprog Hadv]";
+      [assumption|].
+
+    set prog_in_inv :=
+      filter (λ '(a, _), a ∈ minv_dom I) (prog_region P).
+    rewrite (_: prog_region P = prog_in_inv ∪ prog_map).
+    2: { symmetry. apply map_union_filter. }
+    iDestruct (big_sepM_union with "Hprog") as "[Hprog_inv Hprog]".
+    by apply map_disjoint_filter.
+
+    iMod (inv_alloc invN ⊤ (minv_sep I) with "[Hprog_inv]") as "#Hinv".
+    { iNext. unfold minv_sep. iExists prog_in_inv. iFrame. iPureIntro.
+      assert (minv_dom I ⊆ dom (gset Addr) (prog_region P)).
+      { etransitivity. eapply HIdom. rewrite prog_region_dom//. }
+      rewrite filter_dom_is_dom; auto. split; auto.
+      eapply minv_sub_restrict; [ | | eapply HI]. rewrite filter_dom_is_dom//.
+      transitivity (prog_region P); auto. rewrite /prog_in_inv.
+      eapply map_filter_sub; typeclasses eauto. }
+
+    unfold is_initial_registers in Hreg.
+    destruct Hreg as (HPC & Hr0 & Hrothers).
+    iDestruct (big_sepM_delete _ _ PC with "Hreg") as "[HPC Hreg]"; eauto.
+    iDestruct (big_sepM_delete _ _ r_t0 with "Hreg") as "[Hr0 Hreg]".
+      by rewrite lookup_delete_ne //.
+
+    set rmap := delete r_t0 (delete PC reg).
+    iAssert ([∗ map] r↦w ∈ rmap, r ↦ᵣ w ∗ ⌜is_cap w = false⌝)%I
+               with "[Hreg]" as "Hreg".
+    { iApply (big_sepM_mono with "Hreg"). intros r w Hr. cbn.
+      subst rmap. apply lookup_delete_Some in Hr as [? Hr].
+      apply lookup_delete_Some in Hr as [? Hr].
+      feed pose proof (Hrothers r) as HH. set_solver.
+      destruct HH as [? (? & ?)]. simplify_map_eq. iIntros. iFrame. eauto. }
+
+    assert (∀ r, is_Some (reg !! r)) as Hreg_full.
+    { intros r.
+      destruct (decide (r = PC)); subst; [by eauto|].
+      destruct (decide (r = r_t0)); subst; [by eauto|].
+      destruct (Hrothers r) as [? [? ?] ]; eauto. set_solver. }
+
+    iDestruct (mkregion_sepM_to_sepL2 with "Hadv") as "Hadv". apply prog_size.
+    iDestruct (@region_integers_alloc _ memg with "Hadv") as ">Hadv".
+      by eapply Hadv. by assert (PermFlowsTo RO RWX); eauto.
+
+    iPoseProof (Hspec rmap with "[$HPC $Hr0 $Hreg $Hprog $Hadv $Hinv]") as "Spec".
+    { subst rmap. rewrite !dom_delete_L regmap_full_dom. set_solver+. apply Hreg_full. }
+
+    iModIntro.
+    iExists (fun σ κs _ => ((gen_heap_interp σ.1) ∗ (gen_heap_interp σ.2)))%I.
+    iExists (fun _ => True)%I. cbn. iFrame.
+    iIntros "[Hreg' Hmem']". iExists (⊤ ∖ ↑invN).
+    iInv invN as ">Hx" "_".
+    unfold minv_sep. iDestruct "Hx" as (mi) "(Hmi & Hmi_dom & %)".
+    iDestruct "Hmi_dom" as %Hmi_dom.
+    iDestruct (gen_heap_valid_inclSepM with "Hmem' Hmi") as %Hmi_incl.
+    iModIntro. iPureIntro. rewrite /state_is_good //=.
+    eapply minv_sub_extend; [| |eassumption].
+    rewrite Hmi_dom //. auto. auto.
+  Qed.
+
+End Adequacy.
+
+Theorem template_adequacy `{MachineParameters}
+    (P Adv: prog) (I: memory_inv)
+    (m m': Mem) (reg reg': Reg) (es: list cap_lang.expr):
+  is_initial_memory P Adv m →
+  is_initial_registers P Adv reg →
+  Forall (λ w, is_cap w = false) (prog_instrs Adv) →
+  minv I m →
+  minv_dom I ⊆ list_to_set (region_addrs (prog_start P) (prog_end P)) →
+
+  let prog_map := filter (fun '(a, _) => a ∉ minv_dom I) (prog_region P) in
+  (∀ `{memG Σ, regG Σ, logrel_na_invs Σ} rmap,
+   dom (gset RegName) rmap = all_registers_s ∖ {[ PC; r_t0 ]} →
+   ⊢ inv invN (minv_sep I)
+     ∗ PC ↦ᵣ WCap RWX (prog_start P) (prog_end P) (prog_start P)
+     ∗ r_t0 ↦ᵣ WCap RWX (prog_start Adv) (prog_end Adv) (prog_start Adv)
+     ∗ interp (WCap RWX (prog_start Adv) (prog_end Adv) (prog_start Adv))
+     ∗ ([∗ map] r↦w ∈ rmap, r ↦ᵣ w ∗ ⌜is_cap w = false⌝)
+     ∗ ([∗ map] a↦w ∈ prog_map, a ↦ₐ w)
+     -∗ WP Seq (Instr Executable) {{ λ _, True }}) →
+
+  rtc erased_step ([Seq (Instr Executable)], (reg, m)) (es, (reg', m')) →
+  minv I m'.
+Proof.
+  set (Σ := #[invΣ; gen_heapΣ Addr Word; gen_heapΣ RegName Word;
+              na_invΣ]).
+  intros. eapply (@template_adequacy' Σ); eauto; typeclasses eauto.
+Qed.
+
+End with_adv.
